update proof moore2mealy

transformations/Moore2Mealy/Equivalence.v
@@ -5,13 +5,42 @@ Require Import Mealy.
 Require Import MealySemantics.
 Require Import Moore2Mealy.
 Require Import core.Syntax.
+Require Import List.
+Require Import core.Engine.
+Require Import core.modeling.ModelingEngine.
 Require Import core.Semantics.
 Require Import core.utils.Utils.
-Require Import List.
+Require Import core.Model.
+Require Import core.Certification.
+Require Import core.modeling.ConcreteSyntax.
+Require Import core.modeling.ModelingSemantics.
+Require Import core.modeling.ModelingMetamodel.
+Require Import core.modeling.ConcreteExpressions.
+Require Import core.modeling.Parser.
+Require Import core.SyntaxCertification.
+Require Import core.TransformationConfiguration.
+Require Import core.modeling.ModelingTransformationConfiguration.
+Require Import core.TraceLink.
+Require Import Coq.Logic.Eqdep_dec.
+
+
 Scheme Equality for list.
 
+Definition toOb s := toModelElement StateClass s.
+Definition toOb' := toModelElement Mealy.StateClass.
 
-
+(* put in metamodels, auto gen *)
+Lemma mealy_state_convert: 
+forall x s,
+MealyMetamodel_toClass StateClass x = return s ->
+toModelElement StateClass s = x.
+Proof.
+intros.
+unfold MealyMetamodel_toObject .
+destruct x.
+simpl in H.
+destruct (MealyMetamodel_eqEClass_dec mecl_arg StateClass); crush.
+Qed.
 
 Lemma Moore2Mealy_executeFromState_eq :
 forall (m : MooreModel) (i: list string)
@@ -29,31 +58,119 @@ induction inputs.
   (* main induction step *)
   (* fold mr_execute just once *)
   unfold MooreSemantics.executeFromState; fold MooreSemantics.executeFromState.
-  destruct (find
-  (fun t : Moore.Transition => (a =? Moore.Transition_getInput t)%string)
-  (MooreSemantics.State_outTransitions q0 m)) eqn: mr_s_tr_input.
--- destruct (Moore.Transition_getTarget t m) eqn: mr_t_tr_trg.
-    * unfold executeFromState; fold executeFromState.
-    destruct (find (fun t0 : Transition => (a =? Transition_getInput t0)%string)
-    (State_outTransitions q0' (execute Moore2Mealy m))) eqn: ml_t_tr_input.
-    ** destruct (Transition_getTarget t0 (execute Moore2Mealy m)) eqn: ml_t_tr_trg.
-        *** (* assert State_getOutput s = Transition_getOutput t0 *)
-            (* apply induction step IHinputs *)
-            admit.
+  destruct (MooreSemantics.State_acceptTransition q0 m a) eqn: mr_q0_atr.
+  * destruct (Moore.Transition_getTarget t m) eqn: mr_atr_trg.
+    ** unfold executeFromState; fold executeFromState.
+       destruct (State_acceptTransition q0' (execute Moore2Mealy m) a) eqn: ml_q0'_atr.
+       *** destruct (Transition_getTarget t0 (execute Moore2Mealy m)) eqn: ml_atr_trg.
+           **** (* assert State_getOutput s = Transition_getOutput t0 *)
+                (* apply induction step IHinputs *)
+                admit.
+           **** (* contradiction *) admit.
         *** (* contradiction *) admit.
+    ** unfold executeFromState; fold executeFromState. 
+       destruct (State_acceptTransition q0' (execute Moore2Mealy m) a) eqn: ml_q0'_atr.
+       *** destruct (Transition_getTarget t0 (execute Moore2Mealy m)) eqn: ml_atr_trg.
+           **** (* contradiction *) admit.
+           **** auto.
+       *** (* contradiction mr_q0_atr, ml_qo'_atr *) auto.
+  * unfold executeFromState; fold executeFromState.
+    destruct (State_acceptTransition q0' (execute Moore2Mealy m) a) eqn: ml_q0'_atr.
     ** (* contradiction *) admit.
-    * unfold executeFromState; fold executeFromState.
-      destruct (find (fun t0 : Transition => (a =? Transition_getInput t0)%string)
-      (State_outTransitions q0' (execute Moore2Mealy m))) eqn: ml_t_tr_input.
-      ** destruct (Transition_getTarget t0 (execute Moore2Mealy m)) eqn: ml_t_tr_trg.
-        *** (* contradiction *) admit.
-        *** auto.
-      ** auto.
--- unfold executeFromState.
-  destruct (find (fun t : Transition => (a =? Transition_getInput t)%string) (State_outTransitions q0' (execute Moore2Mealy m))) eqn: ml_s_tr_input.
-  --- (* contradiction *) admit.
-  --- auto.
+    ** auto.
+
 Admitted.
+
+
+Lemma Moore2Mealy_initial_state_eq:
+forall (m : MooreModel), 
+initialState (execute Moore2Mealy m) = None ->
+MooreSemantics.initialState m = None.
+Proof. 
+intros m q0_tr.
+Search flat_map.
+unfold initialState in q0_tr.
+unfold MooreSemantics.initialState.
+apply contraposition.   
+Qed.
+
+
+Lemma Moore2Mealy_initial_state_eq:
+forall (m : MooreModel) s, 
+initialState (execute Moore2Mealy m) = Some s ->
+MooreSemantics.initialState m = None -> False.
+Proof. 
+intros m s q0_tr q0.
+assert (In (toOb' s) (allModelElements (execute Moore2Mealy m))).
+      { unfold initialState in q0_tr.  unfold MealyMetamodel_allStates in q0_tr.
+      apply find_some in q0_tr. 
+      destruct q0_tr.
+      unfold MealyMetamodel_toStates in H.
+      apply optionList2List_In in H.
+      apply in_map_iff in H.
+      do 2 destruct H.
+      unfold toOb'.
+      assert ((toModelElement StateClass s) = x). apply mealy_state_convert. auto.
+      rewrite H2.
+      auto.
+      }
+
+      apply in_flat_map in H as [sp H].
+      destruct H.
+      apply in_flat_map in H0 as [r H0].
+      destruct H0.
+
+      destruct sp.
+      * simpl in H0. crush.
+      * destruct sp.
+        (* sp = n::nil *)
+        ** destruct s0.
+          destruct mocl_arg eqn: clz.
+          - simpl in H0.
+            destruct H0.
+            -- rewrite <- H0 in H1. simpl in H1. 
+              destruct H1. 
+                unfold initialState in q0_tr.
+                apply find_some in q0_tr.
+                unfold toOb' in H1.
+                assert (MealyMetamodel_toObject StateClass (BuildState (Moore.State_getName m0)) =
+                MealyMetamodel_toObject StateClass s). crush.
+                apply Mealy_invert in H2.
+                destruct q0_tr.
+                apply eqb_eq in H4.
+                rewrite <- H2 in H4. simpl in H4.
+                unfold MooreSemantics.initialState.
+                apply find_none with (x:=m0) in q0.
+                apply eqb_neq in q0.
+                --- contradiction.
+                --- unfold MooreMetamodel_allStates. 
+                unfold MooreMetamodel_toStates.
+                (* unfold al
+                lTuples in H. *)
+                apply tuples_up_to_n_incl in H.
+                unfold incl in H.
+                apply optionList2List_In_inv.
+                apply in_map_iff.
+                exists (Build_MooreMetamodel_Object Moore.StateClass m0).
+                split.
+                simpl. auto.
+                specialize (H (Build_MooreMetamodel_Object Moore.StateClass m0)).
+                simpl in H.
+                crush.
+                --- inversion H1.
+            -- crush.
+          -  simpl in H0.
+              destruct H0.
+              -- rewrite <- H0 in H1.
+                  simpl in H1.
+                  destruct H1.
+                  --- unfold toOb' in H1. inversion H1.
+                  --- inversion H1.
+              -- inversion H0.
+        ** (* sp = n::mm::nil *)
+           destruct s0.
+           destruct mocl_arg eqn: clz; simpl in H0; inversion H0.
+Qed.
 
 Theorem Moore2Mealy_equivalence :
     forall (m : MooreModel) (i: list string), 
@@ -65,9 +182,9 @@ destruct (MooreSemantics.initialState m) eqn: q0.
 + destruct (initialState (execute Moore2Mealy m)) eqn: q0_tr.
   ++ (* apply Moore2Mealy_executeFromState_eq *)
      admit.
-  ++ (* contradiction *) admit.
+  ++ (* contradiction, apply Moore2Mealy_initial_state_eq *) admit.
 + destruct (initialState (execute Moore2Mealy m)) eqn: q0_tr.
-  ++ (* contradiction *) admit.
+  ++ specialize (Moore2Mealy_initial_state_eq m s q0_tr q0). intro. inversion H.  
   ++ auto.
 Admitted.
 
